proved skip seq refinement laws

src/Prog.v
@@ -8,6 +8,7 @@ From MRC Require Import Tactics.
 From MRC Require Import Model.
 From MRC Require Import Stdppp.
 From MRC Require Import PredCalc.
+From Equations Require Import Equations.
 
 Open Scope stdpp_scope.
 Open Scope refiney_scope.
@@ -20,6 +21,7 @@ Section prog.
   Local Notation formula := (formula (value M)).
   Local Notation final_formula := (final_formula (value M)).
 
+  Unset Elimination Schemes.
   Inductive prog : Type :=
   | PAsgn (xs : list final_variable) (ts: list final_term) `{OfSameLength _ _ xs ts}
   | PSeq (p1 p2 : prog)
@@ -27,6 +29,25 @@ Section prog.
   | PSpec (w : list final_variable) (pre : final_formula) (post : formula)
   | PVar (x : final_variable) (p : prog)
   | PConst (x : final_variable) (p : prog).
+  Set Elimination Schemes.
+
+  Fixpoint prog_ind P :
+    (∀ xs ts H, P (@PAsgn xs ts H)) →
+    (∀ p1 p2, P p1 → P p2 → P (PSeq p1 p2)) →
+    (∀ gcmds, Forall (λ fp, P fp.2) gcmds → P (PIf gcmds)) →
+    (∀ w pre post, P (PSpec w pre post)) →
+    (∀ x p, P p → P (PVar x p)) →
+    (∀ x p, P p → P (PConst x p)) →
+    ∀ p, P p.
+  Proof with auto.
+    intros Hasgn Hseq Hif Hspec Hvar Hcons. destruct p.
+    - apply Hasgn.
+    - apply Hseq; apply prog_ind...
+    - apply Hif. induction gcmds... constructor... apply prog_ind...
+    - apply Hspec.
+    - apply Hvar. apply prog_ind...
+    - apply Hcons. apply prog_ind...
+  Qed.
 
   Fixpoint PVarList (xs : list final_variable) (p : prog) :=
     match xs with
@@ -180,8 +201,8 @@ Section prog.
     let (opens, xs, ts, _) := args in
     mkAsgnArgs opens (x :: xs) (t :: ts) _.
 
-  Definition split_asgn_list (lhs : list final_variable) (rhs : list asgn_rhs_term)
-    `{H : OfSameLength _ _ lhs rhs} : asgn_args :=
+  Definition split_asgn_list (xs : list final_variable) (rhs : list asgn_rhs_term)
+    `{H : OfSameLength _ _ xs rhs} : asgn_args :=
     of_same_length_rect
       id
         (λ rec x t args,
@@ -190,20 +211,20 @@ Section prog.
           | FinalRhsTerm t => asgn_args_with_closed (rec args) x t
           end)
         (mkAsgnArgs [] [] [] _)
-        lhs rhs.
+        xs rhs.
 
-  Lemma split_asgn_list_cons_closed x t lhs rhs
-      `{Hl1 : !OfSameLength lhs rhs} `{Hl2 : !OfSameLength (x :: lhs) (FinalRhsTerm t :: rhs)} :
-    @split_asgn_list (x :: lhs) (FinalRhsTerm t :: rhs) Hl2  =
-    asgn_args_with_closed (@split_asgn_list lhs rhs Hl1) x t.
+  Lemma split_asgn_list_cons_closed x t xs rhs
+      `{Hl1 : !OfSameLength xs rhs} `{Hl2 : !OfSameLength (x :: xs) (FinalRhsTerm t :: rhs)} :
+    @split_asgn_list (x :: xs) (FinalRhsTerm t :: rhs) Hl2  =
+    asgn_args_with_closed (@split_asgn_list xs rhs Hl1) x t.
   Proof.
     unfold split_asgn_list. simpl. repeat f_equiv. apply OfSameLength_pi.
   Qed.
 
-  Lemma split_asgn_list_cons_open x lhs rhs `{!OfSameLength lhs rhs}
-    `{Hl' : !OfSameLength (x :: lhs) (OpenRhsTerm :: rhs)} :
-    @split_asgn_list (x :: lhs) (OpenRhsTerm :: rhs) Hl' =
-    asgn_args_with_open (split_asgn_list lhs rhs) x.
+  Lemma split_asgn_list_cons_open x xs rhs `{!OfSameLength xs rhs}
+    `{Hl' : !OfSameLength (x :: xs) (OpenRhsTerm :: rhs)} :
+    @split_asgn_list (x :: xs) (OpenRhsTerm :: rhs) Hl' =
+    asgn_args_with_open (split_asgn_list xs rhs) x.
   Proof.
     unfold split_asgn_list. simpl. repeat f_equiv. apply OfSameLength_pi.
   Qed.
@@ -221,19 +242,18 @@ Section prog.
       rewrite H0. rewrite <- H. f_equiv. apply OfSameLength_pi.
   Qed.
 
-  Definition PAsgnWithOpens (lhs : list final_variable) (rhs : list asgn_rhs_term)
-                            `{!OfSameLength lhs rhs} : prog :=
-    let (opens, xs, ts, _) := split_asgn_list lhs rhs in
+  Definition PAsgnWithOpens (xs : list final_variable) (rhs : list asgn_rhs_term)
+                            `{!OfSameLength xs rhs} : prog :=
+    let (opens, xs, ts, _) := split_asgn_list xs rhs in
     PVarList opens (PAsgn xs ts).
 
-
-  Lemma PAsgnWithOpens_cons_open x lhs rhs `{!OfSameLength lhs rhs}
-      `{!OfSameLength (x :: lhs) (OpenRhsTerm :: rhs)} :
-    PAsgnWithOpens (x :: lhs) (OpenRhsTerm :: rhs) =
-      PVar x (PAsgnWithOpens lhs rhs).
+  Lemma PAsgnWithOpens_cons_open x xs rhs `{!OfSameLength xs rhs}
+      `{!OfSameLength (x :: xs) (OpenRhsTerm :: rhs)} :
+    PAsgnWithOpens (x :: xs) (OpenRhsTerm :: rhs) =
+      PVar x (PAsgnWithOpens xs rhs).
   Proof.
     simpl. unfold PAsgnWithOpens at 1. erewrite split_asgn_list_cons_open.
-    unfold asgn_args_with_open. destruct (split_asgn_list lhs rhs) eqn:E.
+    unfold asgn_args_with_open. destruct (split_asgn_list xs rhs) eqn:E.
     simpl. unfold PAsgnWithOpens. rewrite E. reflexivity.
   Qed.
 
@@ -242,6 +262,283 @@ Section prog.
   Proof.
     unfold PAsgnWithOpens. rewrite split_asgn_list_no_opens. simpl. reflexivity.
   Qed.
+
+  Lemma PAsgnWithOpens_app_nil_r xs rhs `{!OfSameLength xs rhs} {Hl} :
+    @PAsgnWithOpens (xs ++ []) (rhs ++ []) Hl = PAsgnWithOpens xs rhs.
+  Proof with auto.
+    unfold PAsgnWithOpens.
+    replace (split_asgn_list (xs ++ []) (rhs ++ [])) with (split_asgn_list xs rhs);
+      [reflexivity|].
+    apply rewrite_of_same_length; rewrite app_nil_r; reflexivity.
+  Qed.
+
+  Lemma asgn_opens_with_open x xs rhs `{!OfSameLength xs rhs} :
+    asgn_opens (asgn_args_with_open (split_asgn_list xs rhs) x) =
+      x :: asgn_opens (split_asgn_list xs rhs).
+  Proof.
+    destruct (split_asgn_list xs rhs). simpl. reflexivity.
+  Qed.
+
+  Lemma asgn_opens_with_closed x t xs rhs `{!OfSameLength xs rhs} :
+    asgn_opens (asgn_args_with_closed (split_asgn_list xs rhs) x t) =
+      asgn_opens (split_asgn_list xs rhs).
+  Proof.
+    destruct (split_asgn_list xs rhs). simpl. reflexivity.
+  Qed.
+
+  Lemma asgn_xs_with_open x xs rhs `{!OfSameLength xs rhs} :
+    asgn_xs (asgn_args_with_open (split_asgn_list xs rhs) x) =
+      asgn_xs (split_asgn_list xs rhs).
+  Proof.
+    destruct (split_asgn_list xs rhs). simpl. reflexivity.
+  Qed.
+
+  Lemma asgn_xs_with_closed x t xs rhs `{!OfSameLength xs rhs} :
+    asgn_xs (asgn_args_with_closed (split_asgn_list xs rhs) x t) =
+      x :: asgn_xs (split_asgn_list xs rhs).
+  Proof.
+    destruct (split_asgn_list xs rhs). simpl. reflexivity.
+  Qed.
+
+  Lemma asgn_ts_with_open x xs rhs `{!OfSameLength xs rhs} :
+    asgn_ts (asgn_args_with_open (split_asgn_list xs rhs) x) =
+      asgn_ts (split_asgn_list xs rhs).
+  Proof.
+    destruct (split_asgn_list xs rhs). simpl. reflexivity.
+  Qed.
+
+  Lemma asgn_ts_with_closed x t xs rhs `{!OfSameLength xs rhs} :
+    asgn_ts (asgn_args_with_closed (split_asgn_list xs rhs) x t) =
+      t :: asgn_ts (split_asgn_list xs rhs).
+  Proof.
+    destruct (split_asgn_list xs rhs). simpl. reflexivity.
+  Qed.
+
+  Lemma asgn_opens_submseteq xs rhs `{!OfSameLength xs rhs} :
+    asgn_opens (split_asgn_list xs rhs) ⊆+ xs.
+  Proof with auto.
+    induction_same_length xs rhs as l r; [set_solver|]. apply submseteq_cons_r.
+    assert (Hl:=of_same_length_rest H'). destruct r.
+    - right. erewrite split_asgn_list_cons_open. rewrite asgn_opens_with_open.
+      eexists. split; [reflexivity | apply IH].
+    - left. erewrite split_asgn_list_cons_closed. rewrite asgn_opens_with_closed.
+      apply IH.
+  Qed.
+
+  Lemma asgn_xs_submseteq xs rhs `{!OfSameLength xs rhs} :
+    asgn_xs (split_asgn_list xs rhs) ⊆+ xs.
+  Proof with auto.
+    induction_same_length xs rhs as l r; [set_solver|]. apply submseteq_cons_r.
+    assert (Hl:=of_same_length_rest H'). destruct r.
+    - left. erewrite split_asgn_list_cons_open. rewrite asgn_xs_with_open. apply IH.
+    - right. erewrite split_asgn_list_cons_closed. rewrite asgn_xs_with_closed. eexists.
+      split; [reflexivity | apply IH].
+  Qed.
+
+
+  Lemma asgn_opens_app xs1 rhs1 xs2 rhs2
+    `{!OfSameLength xs1 rhs1} `{!OfSameLength xs2 rhs2}
+    `{!OfSameLength (xs1 ++ xs2) (rhs1 ++ rhs2)} :
+    asgn_opens (split_asgn_list (xs1 ++ xs2) (rhs1 ++ rhs2)) =
+      asgn_opens (split_asgn_list xs1 rhs1) ++ asgn_opens (split_asgn_list xs2 rhs2).
+  Proof with auto.
+    generalize dependent rhs2. generalize dependent xs2.
+    induction_same_length xs1 rhs1 as l1 r1; simpl.
+    - repeat f_equiv. apply OfSameLength_pi.
+    - intros. assert (Hl1:=of_same_length_rest H'). destruct r1.
+      + erewrite split_asgn_list_cons_open. rewrite asgn_opens_with_open.
+        erewrite split_asgn_list_cons_open. rewrite asgn_opens_with_open.
+        erewrite IH. set_solver.
+      + erewrite split_asgn_list_cons_closed. rewrite asgn_opens_with_closed.
+        erewrite split_asgn_list_cons_closed. rewrite asgn_opens_with_closed.
+        erewrite IH...
+  Qed.
+
+  Lemma asgn_xs_app xs1 rhs1 xs2 rhs2
+    `{!OfSameLength xs1 rhs1} `{!OfSameLength xs2 rhs2}
+    `{!OfSameLength (xs1 ++ xs2) (rhs1 ++ rhs2)} :
+    asgn_xs (split_asgn_list (xs1 ++ xs2) (rhs1 ++ rhs2)) =
+      asgn_xs (split_asgn_list xs1 rhs1) ++ asgn_xs (split_asgn_list xs2 rhs2).
+  Proof with auto.
+    generalize dependent rhs2. generalize dependent xs2.
+    induction_same_length xs1 rhs1 as l1 r1; simpl.
+    - repeat f_equiv. apply OfSameLength_pi.
+    - intros. assert (Hl1:=of_same_length_rest H'). destruct r1.
+      + erewrite split_asgn_list_cons_open. rewrite asgn_xs_with_open.
+        erewrite split_asgn_list_cons_open. rewrite asgn_xs_with_open.
+        erewrite IH. set_solver.
+      + erewrite split_asgn_list_cons_closed. rewrite asgn_xs_with_closed.
+        erewrite split_asgn_list_cons_closed. rewrite asgn_xs_with_closed.
+        erewrite IH...
+  Qed.
+
+  Lemma asgn_ts_app xs1 rhs1 xs2 rhs2
+    `{!OfSameLength xs1 rhs1} `{!OfSameLength xs2 rhs2}
+    `{!OfSameLength (xs1 ++ xs2) (rhs1 ++ rhs2)} :
+    asgn_ts (split_asgn_list (xs1 ++ xs2) (rhs1 ++ rhs2)) =
+      asgn_ts (split_asgn_list xs1 rhs1) ++ asgn_ts (split_asgn_list xs2 rhs2).
+  Proof with auto.
+    generalize dependent rhs2. generalize dependent xs2. induction_same_length xs1 rhs1 as l1 r1;
+      simpl.
+    - repeat f_equiv. apply OfSameLength_pi.
+    - intros. assert (Hl1:=of_same_length_rest H'). destruct r1.
+      + erewrite split_asgn_list_cons_open. rewrite asgn_ts_with_open.
+        erewrite split_asgn_list_cons_open. rewrite asgn_ts_with_open.
+        erewrite IH. set_solver.
+      + erewrite split_asgn_list_cons_closed. rewrite asgn_ts_with_closed.
+        erewrite split_asgn_list_cons_closed. rewrite asgn_ts_with_closed.
+        erewrite IH...
+  Qed.
+
+  Lemma elem_of_asgn_opens x xs rhs `{!OfSameLength xs rhs} :
+    NoDup xs →
+    x ∈ asgn_opens (split_asgn_list xs rhs) ↔ (x, OpenRhsTerm) ∈ (xs, rhs).
+  Proof with auto.
+    induction_same_length xs rhs as l r.
+    - simpl. unfold zip_pair_elem_of. pose proof (elem_of_zip_pair_nil x (OpenRhsTerm)).
+      set_solver.
+    - intros. assert (Hl := of_same_length_rest H'). apply NoDup_cons in H as [].
+      destruct (decide (x = l)).
+      2:{ rewrite elem_of_zip_pair_hd_ne... destruct r.
+          - erewrite split_asgn_list_cons_open. rewrite asgn_opens_with_open.
+            rewrite elem_of_cons. rewrite IH... naive_solver.
+          - erewrite split_asgn_list_cons_closed. rewrite asgn_opens_with_closed.
+            rewrite IH... }
+      subst l. destruct r.
+      + erewrite split_asgn_list_cons_open. rewrite asgn_opens_with_open.
+        rewrite elem_of_cons. rewrite IH... rewrite elem_of_zip_pair_hd... split...
+      + erewrite split_asgn_list_cons_closed. rewrite asgn_opens_with_closed.
+        rewrite IH... rewrite elem_of_zip_pair_hd... split; [|discriminate]. intros (i&?&?).
+        simpl in H1, H2. apply elem_of_list_lookup_2 in H1. contradiction.
+  Qed.
+
+  Lemma elem_of_asgn_xs_ts x t xs rhs `{!OfSameLength xs rhs} :
+    NoDup xs →
+    (x, t) ∈ (asgn_xs (split_asgn_list xs rhs), asgn_ts (split_asgn_list xs rhs)) ↔
+      (x, FinalRhsTerm t) ∈ (xs, rhs).
+  Proof with auto.
+    induction_same_length xs rhs as l r.
+    - simpl. unfold zip_pair_elem_of. pose proof (elem_of_zip_pair_nil x t).
+      pose proof (elem_of_zip_pair_nil x (FinalRhsTerm t)). set_solver.
+    - intros. assert (Hl := of_same_length_rest H'). apply NoDup_cons in H as [].
+      destruct (decide (x = l)).
+      2:{ rewrite elem_of_zip_pair_hd_ne... destruct r.
+          - erewrite split_asgn_list_cons_open. rewrite asgn_xs_with_open.
+            rewrite asgn_ts_with_open. rewrite IH...
+          - erewrite split_asgn_list_cons_closed. rewrite asgn_xs_with_closed.
+            rewrite asgn_ts_with_closed. rewrite elem_of_zip_pair_hd_ne... }
+      subst l. destruct r.
+      + erewrite split_asgn_list_cons_open. rewrite asgn_xs_with_open. rewrite asgn_ts_with_open.
+        rewrite IH... rewrite elem_of_zip_pair_hd... split; [|discriminate]. intros (i&?&?).
+        simpl in H1, H2. apply elem_of_list_lookup_2 in H1. contradiction.
+      + erewrite split_asgn_list_cons_closed. rewrite asgn_xs_with_closed.
+        rewrite asgn_ts_with_closed. rewrite (elem_of_zip_pair_hd (FinalRhsTerm t))...
+        split.
+        * intros (i&?). destruct i.
+          -- apply elem_of_zip_pair_hd_indexed in H1 as [_ ?]. subst...
+          -- apply elem_of_zip_pair_tl_indexed in H1. apply elem_of_zip_pair_indexed_inv in H1.
+             rewrite IH in H1... destruct H1 as (j&?&?). simpl in H1.
+             apply elem_of_list_lookup_2 in H1. contradiction.
+        * intros. inversion H1. subst t0. exists 0. split; simpl...
+  Qed.
+
+  Lemma elem_of_asgn_ts_inv t xs rhs `{!OfSameLength xs rhs} :
+    t ∈ asgn_ts (split_asgn_list xs rhs) →
+    ∃ x, (x, t) ∈ (asgn_xs (split_asgn_list xs rhs), (asgn_ts (split_asgn_list xs rhs))).
+  Proof with auto.
+    intros. apply elem_of_list_lookup in H as (i&?).
+    opose proof (lookup_of_same_length_r (asgn_xs (split_asgn_list xs rhs)) H) as (x&?).
+    { apply asgn_of_same_length. }
+    exists x, i. split...
+  Qed.
+
+  Lemma elem_of_asgn_ts t xs rhs `{!OfSameLength xs rhs} :
+    NoDup xs →
+    t ∈ asgn_ts (split_asgn_list xs rhs) ↔
+      ∃ x, (x, t) ∈ (asgn_xs (split_asgn_list xs rhs), (asgn_ts (split_asgn_list xs rhs))).
+  Proof with auto.
+    intros Hnodup. split; [apply elem_of_asgn_ts_inv|].
+    intros (x&?). apply elem_of_asgn_xs_ts in H as [i []]... simpl in H, H0.
+    generalize dependent i. induction_same_length xs rhs as l r; [set_solver|].
+    intros Hnodup ???. assert (Hl:=of_same_length_rest H'). apply NoDup_cons in Hnodup as [].
+    destruct r.
+    + erewrite split_asgn_list_cons_open. rewrite asgn_ts_with_open.
+      destruct i.
+      * simpl in H0. discriminate.
+      * apply IH with (i:=i)...
+    + erewrite split_asgn_list_cons_closed. rewrite asgn_ts_with_closed. destruct i.
+      * simpl in H0. inversion H0. subst. set_solver.
+      * set_unfold. right. eapply IH; [assumption | exact H | exact H0].
+  Qed.
+
+  Lemma asgn_opens_Permutation xs rhs xs' rhs'
+    `{!OfSameLength xs rhs} `{!OfSameLength xs' rhs'} :
+    NoDup xs →
+    NoDup xs' →
+    (xs, rhs) ≡ₚₚ (xs', rhs') →
+    asgn_opens (split_asgn_list xs rhs) ≡ₚ asgn_opens (split_asgn_list xs' rhs').
+  Proof with auto.
+    generalize dependent xs'. generalize dependent rhs'. induction_same_length xs rhs as l r.
+    - apply zip_pair_Permutation_nil_inv_l in H2... destruct H2 as [-> ->]. simpl...
+    - intros. apply NoDup_cons in H as []. assert (Hl:=of_same_length_rest H').
+      apply zip_pair_Permutation_cons_inv_l in H1...
+      destruct H1 as (xs'0&ys'0&xs'1&ys'1&?&?&?&?&?). destruct r.
+      + erewrite split_asgn_list_cons_open. rewrite asgn_opens_with_open.
+        subst. erewrite asgn_opens_app. erewrite split_asgn_list_cons_open.
+        rewrite asgn_opens_with_open. rewrite app_Permutation_comm.
+        simpl. f_equiv. etrans.
+        * apply IH with (xs':=xs'0 ++ xs'1) (rhs':=ys'0 ++ ys'1)...
+          apply NoDup_app in H0 as (?&?&?). apply NoDup_cons in H3 as []. apply NoDup_app.
+          split_and!... intros. apply H1 in H6. set_solver.
+        * erewrite asgn_opens_app. apply Permutation_app_comm.
+      + erewrite split_asgn_list_cons_closed. rewrite asgn_opens_with_closed.
+        subst. erewrite asgn_opens_app. erewrite split_asgn_list_cons_closed.
+        rewrite asgn_opens_with_closed. rewrite app_Permutation_comm.
+        simpl. etrans.
+        * apply IH with (xs':=xs'0 ++ xs'1) (rhs':=ys'0 ++ ys'1)...
+          apply NoDup_app in H0 as (?&?&?). apply NoDup_cons in H3 as []. apply NoDup_app.
+          split_and!... intros. apply H1 in H6. set_solver.
+        * erewrite asgn_opens_app. apply Permutation_app_comm.
+  Qed.
+
+  Lemma asgn_xs_ts_Permutation xs rhs xs' rhs'
+    `{!OfSameLength xs rhs} `{!OfSameLength xs' rhs'} :
+    NoDup xs →
+    NoDup xs' →
+    (xs, rhs) ≡ₚₚ (xs', rhs') →
+    (asgn_xs (split_asgn_list xs rhs), asgn_ts (split_asgn_list xs rhs)) ≡ₚₚ
+      (asgn_xs (split_asgn_list xs' rhs'), asgn_ts (split_asgn_list xs' rhs')).
+  Proof with auto.
+    generalize dependent xs'. generalize dependent rhs'. induction_same_length xs rhs as l r.
+    - apply zip_pair_Permutation_nil_inv_l in H2... destruct H2 as [-> ->]. simpl...
+    - intros. apply NoDup_cons in H as []. assert (Hl:=of_same_length_rest H').
+      apply zip_pair_Permutation_cons_inv_l in H1...
+      destruct H1 as (xs'0&ys'0&xs'1&ys'1&?&?&?&?&?). destruct r.
+      + erewrite split_asgn_list_cons_open. rewrite asgn_xs_with_open. rewrite asgn_ts_with_open.
+        subst.
+        rewrite IH with (xs':=xs'0 ++ xs'1) (rhs':=ys'0 ++ ys'1)...
+        2:{ apply NoDup_app in H0 as [? []]. apply NoDup_cons in H3 as []. apply NoDup_app.
+            split_and!... intros. apply H1 in H6. set_solver. }
+        repeat erewrite asgn_xs_app. repeat erewrite asgn_ts_app.
+        erewrite split_asgn_list_cons_open. rewrite asgn_xs_with_open. rewrite asgn_ts_with_open...
+        Unshelve. typeclasses eauto.
+      + subst. erewrite asgn_xs_app. erewrite asgn_ts_app.
+        repeat erewrite split_asgn_list_cons_closed. repeat erewrite asgn_xs_with_closed.
+        repeat erewrite asgn_ts_with_closed. rewrite zip_pair_Permutation_app_comm.
+        2:{ apply asgn_of_same_length. }
+        2:{ eapply of_same_length_cons. Unshelve. apply asgn_of_same_length. }
+        simpl. apply zip_pair_Permutation_cons.
+        1:{ apply asgn_of_same_length. }
+        1:{ eapply of_same_length_app. Unshelve. all: apply asgn_of_same_length. }
+        rewrite IH with (xs':=xs'1 ++ xs'0) (rhs':=ys'1 ++ ys'0)...
+        2:{ apply NoDup_app in H0 as (?&?&?). apply NoDup_cons in H3 as []. apply NoDup_app.
+            split_and!... intros. intros contra. apply H1 in contra. set_solver. }
+        2:{ rewrite zip_pair_Permutation_app_comm... }
+        erewrite asgn_xs_app. erewrite asgn_ts_app...
+        Unshelve. typeclasses eauto.
+  Qed.
+
+
 End prog.
 
 Declare Custom Entry asgn_rhs_seq.
@@ -353,16 +650,16 @@ Notation "'|[' 'var' x '⦁' y ']|' " :=
 
 Notation "'|[' 'var*' xs '⦁' y ']|' " :=
   (PVarList xs y)
-    (in custom prog at level 95 ) : refiney_scope.
+    (in custom prog at level 95, xs custom variable_list) : refiney_scope.
 
 Notation "'|[' 'con' x '⦁' y ']|' " :=
   (PConst x y)
     (in custom prog at level 95, no associativity,
-        x constr at level 0, y custom prog at next level) : refiney_scope.
+        x constr at level 0, y custom prog) : refiney_scope.
 
 Notation "'|[' 'con*' xs '⦁' y ']|' " :=
   (PConstList xs y)
-    (in custom prog at level 95 ) : refiney_scope.
+    (in custom prog at level 95, xs custom variable_list) : refiney_scope.
 
 Notation "{ A }" := (PSpec [] (as_final_formula A) <! true !>)
                         (in custom prog at level 95, no associativity,
@@ -388,16 +685,62 @@ Section prog.
   Local Notation term := (term value).
   Local Notation formula := (formula value).
   Local Notation final_term := (final_term value).
+  Local Notation final_formula := (final_formula value).
 
   Implicit Types A B C : formula.
   Implicit Types pre post : formula.
   Implicit Types w : list final_variable.
   Implicit Types xs : list final_variable.
 
-  Lemma wp_asgn xs ts A `{OfSameLength _ _ xs ts} :
+  Lemma wp_asgn xs ts A `{!OfSameLength xs ts} :
     wp <{ *xs := *$(FinalRhsTerm <$> ts) }> A ≡ <! A[[ ↑ₓ xs \ ⇑ₜ ts]] !>.
   Proof with auto.
     rewrite PAsgnWithOpens_no_opens. simpl...
   Qed.
+
+  Lemma wp_varlist xs p A :
+    wp <{ |[ var* xs ⦁ $p ]| }> A ≡ <! ∀* ↑ₓ xs, $(wp p A) !>.
+  Proof with auto. induction xs as [|x xs IH]... simpl. rewrite IH. reflexivity. Qed.
+
+  Lemma wp_constlist xs p A :
+    wp <{ |[ con* xs ⦁ $p ]| }> A ≡ <! ∃* ↑ₓ xs, $(wp p A) !>.
+  Proof with auto. induction xs as [|x xs IH]... simpl. rewrite IH. reflexivity. Qed.
+
+  Global Instance PVar_proper : Proper ((=) ==> (≡) ==> (≡@{prog})) PVar.
+  Proof. intros x ? <- A B ? C. simpl. rewrite (H C). reflexivity. Qed.
+
+  Global Instance PVarList_proper : Proper ((=) ==> (≡) ==> (≡@{prog})) PVarList.
+  Proof.
+    intros xs ? <- A B ? C. induction xs as [|x xs IH].
+    - simpl. apply H.
+    - simpl. rewrite IH. reflexivity.
+  Qed.
+
+  Global Instance PConst_proper : Proper ((=) ==> (≡) ==> (≡@{prog})) PConst.
+  Proof. intros x ? <- A B ? C. simpl. rewrite (H C). reflexivity. Qed.
+
+  Global Instance PConstList_proper : Proper ((=) ==> (≡) ==> (≡@{prog})) PConstList.
+  Proof.
+    intros xs ? <- A B ? C. induction xs as [|x xs IH].
+    - simpl. apply H.
+    - simpl. rewrite IH. reflexivity.
+  Qed.
+
+  Global Instance wp_proper_fequiv : Proper ((=) ==> (≡) ==> (≡)) (@wp M).
+  Proof with auto.
+    intros p ? <- A B H. generalize dependent B. generalize dependent A.
+    induction p; intros A B Hequiv; intros; simpl; fSimpl;
+      (try solve [rewrite Hequiv; reflexivity]).
+    - apply IHp1. apply IHp2...
+    - generalize dependent B. generalize dependent A. induction gcmds; intros; simpl...
+      apply Forall_cons in H as []. f_equiv.
+      + rewrite H; [reflexivity | exact Hequiv].
+      + apply IHgcmds...
+    - rewrite IHp; [reflexivity|]...
+    - rewrite IHp; [reflexivity|]...
+  Qed.
+
+  Global Instance wp_proper_pequiv {A : final_formula} : Proper ((≡@{prog}) ==> (≡)) (λ p, wp p A).
+  Proof. intros p1 p2 Hp. specialize (Hp A). assumption. Qed.
 
 End prog.
